SSA/Core/Util/ConcreteOrMVar.lean
@@ -44,7 +44,7 @@ def instantiateOne (a : α) : ConcreteOrMVar α (φ+1) → ConcreteOrMVar α φ
       (fun j => .mvar j)  -- `i = Fin.castSucc j`
 
 /-- Instantiate all meta-variables -/
-def instantiate (as : Mathlib.Vector α φ) : ConcreteOrMVar α φ → α
+def instantiate (as : List.Vector α φ) : ConcreteOrMVar α φ → α
   | .concrete w => w
   | .mvar i => as.get i
 
@@ -54,14 +54,14 @@ def ofNat_eq_concrete (x : Nat) :
     (OfNat.ofNat x) = (ConcreteOrMVar.concrete x : ConcreteOrMVar Nat φ) := rfl
 
 @[simp]
-def instantiate_ofNat_eq (as : Mathlib.Vector Nat φ) (x : Nat) :
+def instantiate_ofNat_eq (as : List.Vector Nat φ) (x : Nat) :
    ConcreteOrMVar.instantiate as (OfNat.ofNat x) = x := rfl
 
 @[simp]
 lemma instantiate_mvar_zero {hφ : List.length (w :: ws) = φ} {h0 : 0 < φ} :
     ConcreteOrMVar.instantiate (Subtype.mk (w :: ws) hφ)  (ConcreteOrMVar.mvar ⟨0, h0⟩) = w := by
   simp [instantiate]
-  simp [Mathlib.Vector.get]
+  simp [List.Vector.get]
 
 @[simp]
 lemma instantiate_mvar_zero' :
